theories/TM/Compound/MoveToSymbol.v
@@ -44,7 +44,7 @@ Section MoveToSymbol.
       match current t1 with
       | Some s => if (f s)
                  then tape_write t1 (Some (g s))
-                 else tape_move_mono t1 (Some (g s), R)
+                 else doAct t1 (Some (g s), R)
       | _ => t1
       end.
 
@@ -95,7 +95,7 @@ Section MoveToSymbol.
     match current t with
     | Some m => if f m
                then tape_write t (Some (g m))
-               else MoveToSymbol_Fun (tape_move_mono t (Some (g m), R))
+               else MoveToSymbol_Fun (doAct t (Some (g m), R))
     | _ => t
     end.
   Proof.
@@ -128,7 +128,7 @@ Section MoveToSymbol.
   Lemma MoveToSymbol_Step_false t x :
     current t = Some x ->
     f x = false ->
-    MoveToSymbol_Step_Fun t = tape_move_mono t (Some (g x), R).
+    MoveToSymbol_Step_Fun t = doAct t (Some (g x), R).
   Proof.
     intros H1 H2. unfold MoveToSymbol_Step_Fun. destruct t; cbn in *; inv H1. rewrite H2. auto.
   Qed.
@@ -144,7 +144,7 @@ Section MoveToSymbol.
   Lemma MoveToSymbol_skip t s :
     current t = Some s ->
     f s = false ->
-    MoveToSymbol_Fun (tape_move_mono t (Some (g s), R)) = MoveToSymbol_Fun t.
+    MoveToSymbol_Fun (doAct t (Some (g s), R)) = MoveToSymbol_Fun t.
   Proof. intros H1 H2. cbn. symmetry. rewrite MoveToSymbol_Fun_equation. cbn. now rewrite H1, H2. Qed.
 
   Definition MoveToSymbol_Rel : Rel (tapes sig 1) (unit * tapes sig 1) :=
@@ -178,7 +178,7 @@ Section MoveToSymbol.
 
   Function MoveToSymbol_steps (t : tape sig) { measure rlength t } : nat :=
     match current t with
-    | Some m => if f m then 4 else 4 + (MoveToSymbol_steps (tape_move_mono t (Some (g m), R)))
+    | Some m => if f m then 4 else 4 + (MoveToSymbol_steps (doAct t (Some (g m), R)))
     | _ => 4
     end.
   Proof.
@@ -206,7 +206,7 @@ Section MoveToSymbol.
           * rewrite MoveToSymbol_steps_equation in HT. rewrite E in HT. omega.
         + destruct (current tin[@Fin0]) eqn:E.
           * destruct (f e) eqn:Ef; inv H0. rewrite MoveToSymbol_steps_equation in HT. rewrite E, Ef in HT.
-            exists (MoveToSymbol_steps (tape_move_mono tin[@Fin0] (Some (g e), R))). cbn.
+            exists (MoveToSymbol_steps (doAct tin[@Fin0] (Some (g e), R))). cbn.
             split.
             -- unfold MoveToSymbol_Step_Fun. rewrite E, Ef. cbn. reflexivity.
             -- rewrite <- HT. cbn. omega.
@@ -227,7 +227,7 @@ Section MoveToSymbol.
     | Some s  =>
       if f s
       then tape_write t (Some (g s))
-      else MoveToSymbol_L_Fun (tape_move_mono t (Some (g s), L))
+      else MoveToSymbol_L_Fun (doAct t (Some (g s), L))
     | _ => t
     end.
   Proof. intros. unfold llength. cbn. simpl_tape. destruct t; cbn in *; inv teq. omega. Qed.
@@ -269,7 +269,7 @@ Section MoveToSymbol.
 
   Function MoveToSymbol_L_steps (t : tape sig) { measure llength t } : nat :=
     match current t with
-    | Some s => if f s then 4 else 4 + (MoveToSymbol_L_steps (tape_move_mono t (Some (g s), L)))
+    | Some s => if f s then 4 else 4 + (MoveToSymbol_L_steps (doAct t (Some (g s), L)))
     | _ => 4
     end.
   Proof. intros. unfold llength. cbn. simpl_tape. destruct t; cbn in *; inv teq. omega. Qed.
